rupicola/stlc/ExpRel.fst
@@ -9,9 +9,8 @@ open QTyp
 
 (** Cross Language Binary Logical Relation between F* and STLC expressions
      for __closed terms__. **)
-let rec (∋) (t:qType) (p:get_Type t * closed_exp) : Tot Type0 (decreases %[get_rel t;0]) =
-  let fs_v = fst p in
-  let e = snd p in
+let rec (∋) (t:qType) (p:fs_val t * closed_exp) : Tot Type0 (decreases %[get_rel t;0]) =
+  let (fs_v, e) = p in
   match get_rel t with // way to "match" on F* types
   | QUnit -> fs_v == () /\ e == EUnit
   | QBool -> (fs_v == true /\ e == ETrue) \/ (fs_v == false /\ e == EFalse)
@@ -36,9 +35,8 @@ let rec (∋) (t:qType) (p:get_Type t * closed_exp) : Tot Type0 (decreases %[get
     | Inr fs_v', EInr e' -> (| s2, r2 |) ∋ (fs_v', e')
     | _ -> False
   end
-and (⦂) (t:qType) (p: get_Type t * closed_exp) : Tot Type0 (decreases %[get_rel t;1]) =
-  let fs_e = fst p in
-  let e = snd p in
+and (⦂) (t:qType) (p: fs_val t * closed_exp) : Tot Type0 (decreases %[get_rel t;1]) =
+  let (fs_e, e) = p in
   forall (e':closed_exp). steps e e' ==> irred e' ==> t ∋ (fs_e, e')
 
 let lem_values_are_expressions t fs_e e : (** lemma used by Amal **)
@@ -63,7 +61,7 @@ let rec lem_values_are_values t fs_e (e:closed_exp) :
     | Inr fs_e', EInr e' -> lem_values_are_values (| s2, r2 |) fs_e' e'
 
 
-let safety (t:qType) (fs_e:get_Type t) (e:closed_exp) : Lemma
+let safety (t:qType) (fs_e:fs_val t) (e:closed_exp) : Lemma
   (requires t ⦂ (fs_e, e))
   (ensures safe e) =
   introduce forall e'. steps e e' ==> is_value e' \/ can_step e' with begin
@@ -98,22 +96,22 @@ let (∽) (#g:typ_env) #b (fsG:eval_env g) (s:gsub g b) : Type0 =
 
 (** Cross Language Binary Logical Relation between F* and STLC expressions
      for __open terms__. **)
-let equiv (#g:typ_env) (t:qType) (fs_e:fs_oexp g t) (e:exp) : Type0 =
+let equiv (#g:typ_env) (t:qType) (fs_e:fs_oval g t) (e:exp) : Type0 =
   fv_in_env g e /\
   forall b (s:gsub g b) (fsG:eval_env g).
     fsG ∽ s ==>  t ⦂ (fs_e fsG, gsubst s e)
 
-let (≈) (#g:typ_env) (#t:qType) (fs_v:fs_oexp g t) (e:exp) : Type0 =
+let (≈) (#g:typ_env) (#t:qType) (fs_v:fs_oval g t) (e:exp) : Type0 =
   equiv #g t fs_v e
 
 (** Equiv closed terms **)
-let equiv_closed_terms (#t:qType) (fs_e:get_Type t) (e:closed_exp) :
+let equiv_closed_terms (#t:qType) (fs_e:fs_val t) (e:closed_exp) :
   Lemma (requires equiv #empty t (fun _ -> fs_e) e)
         (ensures  t ⦂ (fs_e, e)) =
   eliminate forall b (s:gsub empty b) (fsG:eval_env empty).
     fsG ∽ s ==>  t ⦂ ((fun _ -> fs_e) fsG, gsubst s e) with true gsub_empty empty_eval
 
-let lem_equiv_exp_are_equiv (g:typ_env) (#t:qType) (fs_e:get_Type t) (e:closed_exp) :
+let lem_equiv_exp_are_equiv (g:typ_env) (#t:qType) (fs_e:fs_val t) (e:closed_exp) :
   Lemma (requires t ⦂ (fs_e, e))
         (ensures  equiv #empty t (fun _ -> fs_e) e) =
   introduce forall b (s:gsub empty b) (fsG:eval_env empty).
@@ -166,7 +164,7 @@ let equiv_var0 (g:typ_env) (t:qType)
   end
 
 (** Used in compilation **)
-let equiv_varS (#g:typ_env) #a #t (s:fs_oexp g a) (e:exp)
+let equiv_varS (#g:typ_env) #a #t (s:fs_oval g a) (e:exp)
   : Lemma
       (requires (equiv #g a s e))
       (ensures (equiv #(extend t g) a (fun fsG -> s (tail fsG)) (subst sub_inc e)))
@@ -183,7 +181,7 @@ let equiv_var g (x:var{Some? (g x)})
     end
   end
 
-let equiv_lam #g (t1:qType) (t2:qType) (f:fs_oexp g (t1 ^-> t2)) (body:exp) : Lemma
+let equiv_lam #g (#t1:qType) (#t2:qType) (f:fs_oval g (t1 ^-> t2)) (body:exp) : Lemma
   (requires (fun (fsG:eval_env (extend t1 g)) -> f (tail #t1 fsG) (hd fsG)) ≈ body)
   (ensures f ≈ (ELam body)) =
   lem_fv_in_env_lam g t1 body;
@@ -192,7 +190,7 @@ let equiv_lam #g (t1:qType) (t2:qType) (f:fs_oexp g (t1 ^-> t2)) (body:exp) : Le
     introduce _ ==> _ with _. begin
       let body' = subst (sub_elam s) body in
       assert (gsubst s (ELam body) == ELam body');
-      introduce forall (v:value) (fs_v:get_Type t1). t1 ∋ (fs_v, v) ==>  t2 ⦂ (f fsG fs_v, subst_beta v body') with begin
+      introduce forall (v:value) (fs_v:fs_val t1). t1 ∋ (fs_v, v) ==>  t2 ⦂ (f fsG fs_v, subst_beta v body') with begin
         introduce _ ==> _ with _. begin
           let s' = gsub_extend s t1 v in
           let fsG' = stack fsG fs_v in
@@ -218,7 +216,7 @@ let equiv_lam #g (t1:qType) (t2:qType) (f:fs_oexp g (t1 ^-> t2)) (body:exp) : Le
 #push-options "--z3rlimit 5000 --fuel 5000"
 let equiv_app #g
   (#t1:qType) (#t2:qType)
-  (fs_e1:fs_oexp g (t1 ^-> t2)) (fs_e2:fs_oexp g t1)
+  (fs_e1:fs_oval g (t1 ^-> t2)) (fs_e2:fs_oval g t1)
   (e1:exp) (e2:exp)
   : Lemma
     (requires fs_e1 ≈ e1 /\ fs_e2 ≈ e2)
@@ -247,7 +245,7 @@ let equiv_app #g
               assert (steps e2 e2');
               assert (irred e2')
             end;
-            eliminate forall (v:value) (fs_v:get_Type t1). t1 ∋ (fs_v, v) ==>
+            eliminate forall (v:value) (fs_v:fs_val t1). t1 ∋ (fs_v, v) ==>
               t2 ⦂ (fs_e1 fs_v, subst_beta v e11)
             with e2' fs_e2;
             assert (t2 ⦂ (fs_e, subst_beta e2' e11));
@@ -258,7 +256,7 @@ let equiv_app #g
     end
   end
 
-let equiv_if #g (#t:qType) (fs_e1:fs_oexp g qBool) (fs_e2:fs_oexp g t) (fs_e3:fs_oexp g t) (e1:exp) (e2:exp) (e3:exp) : Lemma
+let equiv_if #g (#t:qType) (fs_e1:fs_oval g qBool) (fs_e2:fs_oval g t) (fs_e3:fs_oval g t) (e1:exp) (e2:exp) (e3:exp) : Lemma
   (requires fs_e1 ≈ e1 /\ fs_e2 ≈ e2 /\ fs_e3 ≈ e3)
   (ensures (fun fsG -> if fs_e1 fsG then fs_e2 fsG else fs_e3 fsG) ≈ EIf e1 e2 e3) =
   lem_fv_in_env_if g e1 e2 e3;
@@ -288,7 +286,7 @@ let equiv_if #g (#t:qType) (fs_e1:fs_oexp g qBool) (fs_e2:fs_oexp g t) (fs_e3:fs
   end
 #pop-options
 
-let equiv_pair #g (#t1 #t2:qType) (fs_e1:fs_oexp g t1) (fs_e2:fs_oexp g t2) (e1:exp) (e2:exp) : Lemma
+let equiv_pair #g (#t1 #t2:qType) (fs_e1:fs_oval g t1) (fs_e2:fs_oval g t2) (e1:exp) (e2:exp) : Lemma
   (requires fs_e1 ≈ e1 /\ fs_e2 ≈ e2)
   (ensures (fun fsG -> (fs_e1 fsG, fs_e2 fsG)) `equiv (t1 ^* t2)` EPair e1 e2) =
   lem_fv_in_env_pair g e1 e2;
@@ -318,7 +316,7 @@ let equiv_pair #g (#t1 #t2:qType) (fs_e1:fs_oexp g t1) (fs_e2:fs_oexp g t2) (e1:
     end
   end
 
-let equiv_pair_fst_app #g (#t1 #t2:qType) (fs_e12:fs_oexp g (t1 ^* t2)) (e12:exp) : Lemma
+let equiv_pair_fst_app #g (#t1 #t2:qType) (fs_e12:fs_oval g (t1 ^* t2)) (e12:exp) : Lemma
   (requires fs_e12 `equiv (t1 ^* t2)` e12) (** is this too strict? we only care for the left to be equivalent. **)
   (ensures (fun fsG -> fst (fs_e12 fsG)) `equiv t1` (EFst e12)) =
   introduce forall b (s:gsub g b) fsG. fsG ∽ s ==>  t1 ⦂ (fst (fs_e12 fsG), gsubst s (EFst e12)) with begin
@@ -384,7 +382,7 @@ let equiv_pair_fst g (t1 t2:qType)
     assert (t ⦂ (fs_e, e))
   end
 
-let equiv_pair_snd_app #g (#t1 #t2:qType) (fs_e12:fs_oexp g (t1 ^* t2)) (e12:exp)
+let equiv_pair_snd_app #g (#t1 #t2:qType) (fs_e12:fs_oval g (t1 ^* t2)) (e12:exp)
   : Lemma
     (requires fs_e12 `equiv (t1 ^* t2)` e12) (** is this too strict? we only care for the left to be equivalent. **)
     (ensures (fun fsG -> snd (fs_e12 fsG)) `equiv t2` (ESnd e12))
@@ -432,7 +430,7 @@ let equiv_pair_snd g (t1 t2:qType)
 
     eliminate True /\ True
     returns t ∋ (fs_e, e) with _ _. begin
-      introduce forall (v:value) (fs_v:get_Type tp). tp ∋ (fs_v, v) ==>
+      introduce forall (v:value) (fs_v:fs_val tp). tp ∋ (fs_v, v) ==>
         t2 ⦂ (fs_e fs_v, subst_beta v (ESnd (EVar 0))) with begin
         introduce _ ==> _ with _. begin
           lem_values_are_expressions tp fs_v v;
