rupicola/stlc/Examples.fst
@@ -6,16 +6,16 @@ let ut_unit = ()
 let ut_true = true
 let ut_false = false
 
-val var0 : fs_oexp (extend qBool empty) qBool
+val var0 : fs_oval (extend qBool empty) qBool
 let var0 fsG = hd fsG
 
-val var1 : fs_oexp (extend qBool (extend qBool empty)) qBool
+val var1 : fs_oval (extend qBool (extend qBool empty)) qBool
 let var1 fsG = hd (tail fsG)
 
-let var2 : fs_oexp (extend qBool (extend qBool (extend qBool empty))) qBool =
+let var2 : fs_oval (extend qBool (extend qBool (extend qBool empty))) qBool =
   fun fsG -> hd (tail (tail fsG))
 
-let var3 : fs_oexp (extend qBool (extend qBool (extend qBool (extend qBool empty)))) qBool =
+let var3 : fs_oval (extend qBool (extend qBool (extend qBool (extend qBool empty)))) qBool =
   fun fsG -> hd (tail (tail (tail fsG)))
 
 let constant (x: bool) : bool =
