rupicola/stlc/QExp.fst
@@ -10,53 +10,53 @@ unfold
 val helper_var0 :
   g:typ_env ->
   a:qType ->
-  fs_oexp (extend a g) a
+  fs_oval (extend a g) a
 let helper_var0 g a fsG = hd fsG
 
 unfold
 val helper_varS : g:typ_env ->
                   a:qType ->
                   b:qType ->
-                  fs_oexp g a ->
-                  fs_oexp (extend b g) a
+                  fs_oval g a ->
+                  fs_oval (extend b g) a
 let helper_varS g a b x fsG = x (tail fsG)
 
 unfold
-val helper_unit : g:typ_env -> fs_oexp g qUnit
+val helper_unit : g:typ_env -> fs_oval g qUnit
 let helper_unit g _ = ()
 
 unfold
 val helper_app: #g : typ_env ->
                 #a : qType ->
                 #b : qType ->
-                f :fs_oexp g (a ^-> b) ->
-                x :fs_oexp g a ->
-                fs_oexp g b
+                f :fs_oval g (a ^-> b) ->
+                x :fs_oval g a ->
+                fs_oval g b
 let helper_app f x fsG = (f fsG) (x fsG)
 
 unfold
 val helper_lambda : #g :typ_env ->
                 #a :qType ->
                 #b :qType ->
-                f :fs_oexp g (a ^-> b) ->
-                fs_oexp (extend a g) b
+                f :fs_oval g (a ^-> b) ->
+                fs_oval (extend a g) b
 let helper_lambda #_ #_ f fsG = f (tail fsG) (hd fsG)
 
 unfold
-val helper_true : g:typ_env -> fs_oexp g qBool
+val helper_true : g:typ_env -> fs_oval g qBool
 let helper_true g _ = true
 
 unfold
-val helper_false : g:typ_env -> fs_oexp g qBool
+val helper_false : g:typ_env -> fs_oval g qBool
 let helper_false g _ = false
 
 unfold
 val helper_if : #g :typ_env ->
                 #a  : qType ->
-                c   : fs_oexp g qBool ->
-                t   : fs_oexp g a ->
-                e   : fs_oexp g a ->
-                fs_oexp g a
+                c   : fs_oval g qBool ->
+                t   : fs_oval g a ->
+                e   : fs_oval g a ->
+                fs_oval g a
 let helper_if c t e fsG =
   if c fsG then t fsG else e fsG
 
@@ -64,9 +64,9 @@ unfold
 val helper_pair : #g : typ_env ->
                   #a : qType ->
                   #b : qType ->
-                  x : fs_oexp g a ->
-                  y : fs_oexp g b ->
-                  fs_oexp g (a ^* b)
+                  x : fs_oval g a ->
+                  y : fs_oval g b ->
+                  fs_oval g (a ^* b)
 let helper_pair #_ #_ #_ x y fsG =
   (x fsG, y fsG)
 
@@ -74,32 +74,32 @@ unfold
 val helper_fst : #g : typ_env ->
                  #a : qType ->
                  #b : qType ->
-                 p : fs_oexp g (a ^* b) ->
-                 fs_oexp g a
+                 p : fs_oval g (a ^* b) ->
+                 fs_oval g a
 let helper_fst p fsG = fst (p fsG)
 
 unfold
 val helper_snd : #g : typ_env ->
                  #a : qType ->
                  #b : qType ->
-                 p : fs_oexp g (a ^* b) ->
-                 fs_oexp g b
+                 p : fs_oval g (a ^* b) ->
+                 fs_oval g b
 let helper_snd p fsG = snd (p fsG)
 
 unfold
 val helper_inl : #g : typ_env ->
                  #a : qType ->
                  b : qType ->
-                 p : fs_oexp g a ->
-                 fs_oexp g (a ^+ b)
+                 p : fs_oval g a ->
+                 fs_oval g (a ^+ b)
 let helper_inl _ p fsG = Inl (p fsG)
 
 unfold
 val helper_inr : #g : typ_env ->
                  a : qType ->
                  #b : qType ->
-                 p : fs_oexp g b ->
-                 fs_oexp g (a ^+ b)
+                 p : fs_oval g b ->
+                 fs_oval g (a ^+ b)
 let helper_inr _ p fsG = Inr (p fsG)
 
 unfold
@@ -107,10 +107,10 @@ val helper_case : #g :typ_env ->
                   #a  : qType ->
                   #b  : qType ->
                   #c  : qType ->
-                  cond: fs_oexp g (a ^+ b) ->
-                  inlc: fs_oexp g (a ^-> c) ->
-                  inrc: fs_oexp g (b ^-> c) ->
-                  fs_oexp g c
+                  cond: fs_oval g (a ^+ b) ->
+                  inlc: fs_oval g (a ^-> c) ->
+                  inrc: fs_oval g (b ^-> c) ->
+                  fs_oval g c
 let helper_case cond inlc inrc fsG =
   match cond fsG with
   | Inl x -> inlc fsG x
@@ -118,169 +118,171 @@ let helper_case cond inlc inrc fsG =
 
 [@@no_auto_projectors] // FStarLang/FStar#3986
 noeq
-type exp_quotation : #a:qType -> g:typ_env -> fs_oexp g a -> Type =
-| Qtt         : #g : typ_env -> exp_quotation g (helper_unit g)
+type value_quotation : #a:qType -> g:typ_env -> fs_oval g a -> Type =
+| Qtt         : #g : typ_env -> value_quotation g (helper_unit g)
 
 | QVar0       : #g : typ_env ->
                 #a : qType ->
-                exp_quotation (extend a g) (helper_var0 g a)
+                value_quotation (extend a g) (helper_var0 g a)
 
 | QVarS       : #g : typ_env ->
                 #a : qType ->
                 #b : qType ->
-                #x : fs_oexp g a ->
-                exp_quotation g x ->
-                exp_quotation (extend b g) (helper_varS g a b x)
+                #x : fs_oval g a ->
+                value_quotation g x ->
+                value_quotation (extend b g) (helper_varS g a b x)
 
 | QAppGhost   : #g : typ_env ->
                 #a : qType ->
-                #f : fs_oexp g (a ^-> qUnit) -> (** This has to be Tot. If it is GTot unit, F* can treat it as Pure unit **)
-                #x : fs_oexp g a ->
-                exp_quotation #qUnit g (helper_app #_ #_ #_ f x)
+                #f : fs_oval g (a ^-> qUnit) -> (** This has to be Tot. If it is GTot unit, F* can treat it as Pure unit **)
+                #x : fs_oval g a ->
+                value_quotation #qUnit g (helper_app #_ #_ #_ f x)
 
 | QApp        : #g : typ_env ->
                 #a : qType ->
                 #b : qType ->
-                #f : fs_oexp g (a ^-> b) ->
-                #x : fs_oexp g a ->
-                exp_quotation g f ->
-                exp_quotation g x ->
-                exp_quotation g (helper_app #_ #_ #_ f x)
+                #f : fs_oval g (a ^-> b) ->
+                #x : fs_oval g a ->
+                value_quotation g f ->
+                value_quotation g x ->
+                value_quotation g (helper_app #_ #_ #_ f x)
 
 | QLambda     : #g : typ_env ->
                 #a : qType ->
                 #b : qType ->
-                #f : fs_oexp g (a ^-> b) ->
-                exp_quotation (extend a g) (helper_lambda f) ->
-                exp_quotation g f
+                #f : fs_oval g (a ^-> b) ->
+                value_quotation (extend a g) (helper_lambda f) ->
+                value_quotation g f
 
-| QTrue       : #g : typ_env -> exp_quotation g (helper_true g)
-| QFalse      : #g : typ_env -> exp_quotation g (helper_false g)
+| QTrue       : #g : typ_env -> value_quotation g (helper_true g)
+| QFalse      : #g : typ_env -> value_quotation g (helper_false g)
 | QIf         : #g : typ_env ->
                 #a : qType ->
-                #c : fs_oexp g qBool ->
-                exp_quotation g c ->
-                #t : fs_oexp g a ->
-                exp_quotation g t ->
-                #e : fs_oexp g a ->
-                exp_quotation g e ->
-                exp_quotation g (helper_if c t e)
+                #c : fs_oval g qBool ->
+                value_quotation g c ->
+                #t : fs_oval g a ->
+                value_quotation g t ->
+                #e : fs_oval g a ->
+                value_quotation g e ->
+                value_quotation g (helper_if c t e)
 
 | QMkpair   : #g : typ_env ->
               #a : qType ->
               #b : qType ->
-              #x : fs_oexp g a ->
-              #y : fs_oexp g b ->
-              exp_quotation g x ->
-              exp_quotation g y ->
-              exp_quotation g (helper_pair x y)
+              #x : fs_oval g a ->
+              #y : fs_oval g b ->
+              value_quotation g x ->
+              value_quotation g y ->
+              value_quotation g (helper_pair x y)
 | QFst      : #g : typ_env ->
               #a : qType ->
               #b : qType ->
-              #p : fs_oexp g (a ^* b) ->
-              exp_quotation g p ->
-              exp_quotation g (helper_fst p)
+              #p : fs_oval g (a ^* b) ->
+              value_quotation g p ->
+              value_quotation g (helper_fst p)
 | QSnd      : #g : typ_env ->
               #a : qType ->
               #b : qType ->
-              #p : fs_oexp g (a ^* b) ->
-              exp_quotation g p ->
-              exp_quotation g (helper_snd p)
+              #p : fs_oval g (a ^* b) ->
+              value_quotation g p ->
+              value_quotation g (helper_snd p)
 | QInl      : #g : typ_env ->
               #a : qType ->
               #b : qType ->
-              #p : fs_oexp g a ->
-              exp_quotation g p ->
-              exp_quotation g (helper_inl b p)
+              #p : fs_oval g a ->
+              value_quotation g p ->
+              value_quotation g (helper_inl b p)
 | QInr      : #g : typ_env ->
               #a : qType ->
               #b : qType ->
-              #p : fs_oexp g b ->
-              exp_quotation g p ->
-              exp_quotation g (helper_inr a p)
+              #p : fs_oval g b ->
+              value_quotation g p ->
+              value_quotation g (helper_inr a p)
 | QCase     : #g : typ_env ->
               #a : qType ->
               #b : qType ->
               #c : qType ->
-              #cond : fs_oexp g (a ^+ b) ->
-              exp_quotation g cond ->
-              #inlc : fs_oexp g (a ^-> c) ->
-              exp_quotation g inlc ->
-              #inrc : fs_oexp g (b ^-> c) ->
-              exp_quotation g inrc ->
-              exp_quotation g (helper_case cond inlc inrc)
+              #cond : fs_oval g (a ^+ b) ->
+              value_quotation g cond ->
+              #inlc : fs_oval g (a ^-> c) ->
+              value_quotation g inlc ->
+              #inrc : fs_oval g (b ^-> c) ->
+              value_quotation g inrc ->
+              value_quotation g (helper_case cond inlc inrc)
 
+let (⊢) (#a:qType) (g:typ_env) (x:fs_oval g a) =
+  value_quotation g x
 
 unfold
-let helper_oexp (#a:qType) (x:get_Type a) : fs_oexp empty a = fun _ -> x
+let helper_oexp (#a:qType) (x:get_Type a) : fs_oval empty a = fun _ -> x
 
-type closed_exp_quotation (a:qType) (x:get_Type a) =
-  exp_quotation #a empty (helper_oexp x)
+let (⊩) (a:qType) (x:get_Type a) =
+  value_quotation #a empty (helper_oexp x)
 
 open Examples
 
 #push-options "--no_smt"
 
 let test_ut_unit
-  : closed_exp_quotation qUnit ut_unit
+  : qUnit ⊩ ut_unit
   = Qtt
 
 let test_ut_true
-  : closed_exp_quotation qBool ut_true
+  : qBool ⊩ ut_true
   = QTrue
 
 let test_ut_false
-  : closed_exp_quotation qBool ut_false
+  : qBool ⊩ ut_false
   = QFalse
 
 let test_var0
-  : exp_quotation #qBool (extend qBool empty) var0
+  : (extend qBool empty) ⊢ var0
   = QVar0
 
-let qVar1 #g #a #b : exp_quotation (extend b (extend a g)) (fun fsG -> hd (tail fsG)) =
+let qVar1 #g #a #b : (extend b (extend a g)) ⊢ (fun fsG -> hd (tail fsG)) =
   QVarS QVar0
 
-let qVar2 #g #a #b #c : exp_quotation (extend c (extend b (extend a g))) (fun fsG -> hd (tail (tail fsG))) =
+let qVar2 #g #a #b #c : (extend c (extend b (extend a g))) ⊢ (fun fsG -> hd (tail (tail fsG))) =
   QVarS qVar1
 
 let test_var1
-  : exp_quotation #qBool (extend qBool (extend qBool empty)) var1
+  : (extend qBool (extend qBool empty)) ⊢ var1
   = qVar1
 
 let test_var2
-  : exp_quotation #qBool (extend qBool (extend qBool (extend qBool empty))) var2
+  : (extend qBool (extend qBool (extend qBool empty))) ⊢ var2
   = qVar2
 
 let test_var3
-  : exp_quotation #qBool (extend qBool (extend qBool (extend qBool (extend qBool empty)))) var3
+  : (extend qBool (extend qBool (extend qBool (extend qBool empty)))) ⊢ var3
   = QVarS (qVar2)
 
 let test_constant
-  : closed_exp_quotation (qBool ^-> qBool) constant
+  : (qBool ^-> qBool) ⊩ constant
   = QLambda QTrue
 
 let test_identity
-  : closed_exp_quotation (qBool ^-> qBool) identity
+  : (qBool ^-> qBool) ⊩ identity
   = QLambda QVar0
 
 let test_thunked_id
-  : closed_exp_quotation (qBool ^-> (qBool ^-> qBool)) thunked_id
+  : (qBool ^-> (qBool ^-> qBool)) ⊩ thunked_id
   = QLambda (QLambda QVar0)
 
 let test_proj1
-  : closed_exp_quotation (qBool ^-> qBool ^-> qBool ^-> qBool) proj1
+  : (qBool ^-> qBool ^-> qBool ^-> qBool) ⊩ proj1
   = QLambda (QLambda (QLambda qVar2))
 
 let test_proj2
-  : closed_exp_quotation (qBool ^-> qBool ^-> qBool ^-> qBool) proj2
+  : (qBool ^-> qBool ^-> qBool ^-> qBool) ⊩ proj2
   = QLambda (QLambda (QLambda qVar1))
 
 let test_proj3
-  : closed_exp_quotation (qBool ^-> qBool ^-> qBool ^-> qBool) proj3
+  : (qBool ^-> qBool ^-> qBool ^-> qBool) ⊩ proj3
   = QLambda (QLambda (QLambda QVar0))
 
 let test_apply_top_level_def
-  : closed_exp_quotation (qBool ^-> qBool) apply_top_level_def
+  : (qBool ^-> qBool) ⊩ apply_top_level_def
   = QLambda (QApp
               (QApp
                 (QLambda #_ #_ #_ #(fun _ x y -> y) (QLambda QVar0))
@@ -288,7 +290,7 @@ let test_apply_top_level_def
               QTrue)
 
 let test_apply_top_level_def'
-  : closed_exp_quotation (qBool ^-> qBool ^-> qBool) apply_top_level_def'
+  : (qBool ^-> qBool ^-> qBool) ⊩ apply_top_level_def'
   = QLambda (QLambda (QApp
                        (QApp
                           (QLambda (QLambda #_ #_ #_ #(fun _ y -> y) QVar0))
@@ -297,39 +299,39 @@ let test_apply_top_level_def'
                        QVar0))
 
 let test_papply__top_level_def
-  : closed_exp_quotation (qBool ^-> qBool ^-> qBool) papply__top_level_def
+  : (qBool ^-> qBool ^-> qBool) ⊩ papply__top_level_def
   = QLambda (QApp
               (QLambda #_ #_ #_ #(fun _ x y -> y) (QLambda QVar0))
               QVar0)
 
 let test_apply_arg
-  : closed_exp_quotation ((qUnit ^-> qUnit) ^-> qUnit) apply_arg
+  : ((qUnit ^-> qUnit) ^-> qUnit) ⊩ apply_arg
   = QLambda (QApp QVar0 Qtt)
 
 let test_apply_arg2
-  : closed_exp_quotation ((qBool ^-> qBool ^-> qBool) ^-> qBool) apply_arg2
+  : ((qBool ^-> qBool ^-> qBool) ^-> qBool) ⊩ apply_arg2
   = QLambda (QApp (QApp QVar0 QTrue) QFalse)
 
 
 [@expect_failure]
 let test_proj2'
-  : closed_exp_quotation (qBool ^-> qBool ^-> qBool ^-> qBool) proj2
+  : (qBool ^-> qBool ^-> qBool ^-> qBool) ⊩ proj2
   = QLambda (QLambda (QLambda QVar0))
 
 let test_anif
-  : closed_exp_quotation qBool anif
+  : qBool ⊩ anif
   = QIf QTrue QFalse QTrue
 
 let test_negb
-  : closed_exp_quotation (qBool ^-> qBool) negb
+  : (qBool ^-> qBool) ⊩ negb
   = QLambda (QIf QVar0 QFalse QTrue)
 
 let test_negb_pred
-  : closed_exp_quotation ((qBool ^-> qBool) ^-> qBool ^-> qBool) negb_pred
+  : ((qBool ^-> qBool) ^-> qBool ^-> qBool) ⊩ negb_pred
   = QLambda (QLambda (QIf (QApp qVar1 QVar0) QFalse QTrue))
 
 let test_if2
-  : closed_exp_quotation (qBool ^-> qBool ^-> qBool) if2
+  : (qBool ^-> qBool ^-> qBool) ⊩ if2
   = QLambda (QLambda (QIf qVar1 QFalse QVar0))
 
 (** Because of the fancy types, now one needs a preprocessing tactic to
@@ -337,32 +339,32 @@ let test_if2
 
 let simplify_qType (x:term) : Tac term =
   (** TODO: why is F* not doing this automatically anyway? **)
-  norm_term_env (top_env ()) [delta_only [`%fs_oexp; `%qUnit; `%qBool; `%op_Hat_Subtraction_Greater; `%op_Hat_Star; `%op_Hat_Plus; `%get_rel; `%get_Type; `%Mkdtuple2?._1;`%Mkdtuple2?._2];iota;simplify] x
+  norm_term_env (top_env ()) [delta_only [`%fs_oval; `%qUnit; `%qBool; `%op_Hat_Subtraction_Greater; `%op_Hat_Star; `%op_Hat_Plus; `%get_rel; `%get_Type; `%Mkdtuple2?._1;`%Mkdtuple2?._2];iota;simplify] x
 
 [@@ (preprocess_with simplify_qType)]
 let test_callback_return
-  : closed_exp_quotation (qBool ^-> (qBool ^-> qBool)) callback_return
+  : (qBool ^-> (qBool ^-> qBool)) ⊩ callback_return
   = QLambda (QIf QVar0
                  (QLambda #_ #_ #_ #(fun fsG y -> hd fsG) qVar1)
                  (QLambda #_ #_ #_ #(fun fsG z -> z) QVar0))
 
 [@@ (preprocess_with simplify_qType)]
 let test_callback_return'
-  : closed_exp_quotation (qBool ^-> (qBool ^-> qBool)) callback_return'
+  : (qBool ^-> (qBool ^-> qBool)) ⊩ callback_return'
   = QLambda (QIf QVar0
                  (QLambda #_ #_ #_ #(fun fsG y -> hd fsG) qVar1)
                  (QLambda #_ #_ #_ #(fun fsG -> identity) QVar0)) // TODO: why does it not work to unfold identity here?
 
 let test_make_pair
-  : closed_exp_quotation (qBool ^-> qBool ^-> (qBool ^* qBool)) make_pair
+  : (qBool ^-> qBool ^-> (qBool ^* qBool)) ⊩ make_pair
   = QLambda (QLambda (QMkpair qVar1 QVar0))
 
 [@@ (preprocess_with simplify_qType)]
 let test_pair_of_functions ()
-  : Tot (closed_exp_quotation ((qBool ^-> qBool) ^* (qBool ^-> qBool ^-> qBool))
-                              pair_of_functions)
+  : Tot (((qBool ^-> qBool) ^* (qBool ^-> qBool ^-> qBool))
+                            ⊩ pair_of_functions)
   by (norm [delta_only [`%pair_of_functions]];
-      norm [delta_only [`%fs_oexp; `%qUnit; `%qBool; `%op_Hat_Subtraction_Greater; `%op_Hat_Star; `%get_rel; `%get_Type; `%Mkdtuple2?._1;`%Mkdtuple2?._2];iota];
+      norm [delta_only [`%fs_oval; `%qUnit; `%qBool; `%op_Hat_Subtraction_Greater; `%op_Hat_Star; `%get_rel; `%get_Type; `%Mkdtuple2?._1;`%Mkdtuple2?._2];iota];
      // trefl (); //TODO: why does this fail?
      tadmit ())
   =  QMkpair
@@ -372,44 +374,43 @@ let test_pair_of_functions ()
       (QLambda (QLambda #_ #_ #_ #(fun _ y -> y) QVar0))
 
 let test_pair_of_functions2
-  : closed_exp_quotation
-    ((qBool ^-> qBool) ^* (qBool ^-> qBool ^-> qBool))
-    pair_of_functions2
+  : (((qBool ^-> qBool) ^* (qBool ^-> qBool ^-> qBool))
+    ⊩ pair_of_functions2)
   = admit (); QMkpair // TODO
       (QLambda (QIf QVar0 QFalse QTrue))
       (QLambda (QLambda (QIf qVar1 QFalse QVar0)))
 
 let test_fst_pair
-  : closed_exp_quotation (qBool) fst_pair
+  : (qBool) ⊩ fst_pair
   = (QFst (QMkpair QTrue Qtt))
 
 let test_wrap_fst
-  : closed_exp_quotation ((qBool ^* qBool) ^-> qBool) wrap_fst
+  : ((qBool ^* qBool) ^-> qBool) ⊩ wrap_fst
   = QLambda (QFst QVar0)
 
 let test_wrap_fst_pa
-  : closed_exp_quotation ((qBool ^* qBool) ^-> qBool) wrap_fst_pa
+  : ((qBool ^* qBool) ^-> qBool) ⊩ wrap_fst_pa
   = QLambda (QFst QVar0)
 
 let test_snd_pair
-  : closed_exp_quotation (qUnit) snd_pair
+  : (qUnit) ⊩ snd_pair
   = (QSnd (QMkpair QTrue Qtt))
 
 let test_wrap_snd
-  : closed_exp_quotation ((qBool ^* qUnit) ^-> qUnit) wrap_snd
+  : ((qBool ^* qUnit) ^-> qUnit) ⊩ wrap_snd
   = QLambda (QSnd QVar0)
 
 let test_wrap_snd_pa
-  : closed_exp_quotation ((qBool ^* qUnit) ^-> qUnit) wrap_snd_pa
+  : ((qBool ^* qUnit) ^-> qUnit) ⊩ wrap_snd_pa
   = QLambda (QSnd QVar0)
 
-let qLet #g (#a #b:qType) (#x:fs_oexp g a) (#f:fs_oexp g (a ^-> b))
-  (qx : exp_quotation g x) (qf : exp_quotation g f) :
-  exp_quotation g (fun fsG -> let y = x fsG in f fsG y) =
+let qLet #g (#a #b:qType) (#x:fs_oval g a) (#f:fs_oval g (a ^-> b))
+  (qx : value_quotation g x) (qf : value_quotation g f) :
+  value_quotation g (fun fsG -> let y = x fsG in f fsG y) =
   QApp qf qx
 
 let test_a_few_lets
-  : closed_exp_quotation (qBool ^-> qUnit) a_few_lets
+  : (qBool ^-> qUnit) ⊩ a_few_lets
   = QLambda
      (qLet (QMkpair QVar0 QVar0) (QLambda
      (qLet qVar1 (QLambda
@@ -418,35 +419,35 @@ let test_a_few_lets
      Qtt))))))))
 
 let test_inl_true
-  : closed_exp_quotation (qBool ^+ qUnit) inl_true
+  : (qBool ^+ qUnit) ⊩ inl_true
   = QInl QTrue
 
 let test_inr_unit
-  : closed_exp_quotation (qBool ^+ qUnit) inr_unit
+  : (qBool ^+ qUnit) ⊩ inr_unit
   = QInr Qtt
 
 [@@ (preprocess_with simplify_qType)]
 let test_return_either ()
-  : closed_exp_quotation (qBool ^-> (qUnit ^+ qUnit)) return_either
+  : (qBool ^-> (qUnit ^+ qUnit)) ⊩ return_either
   by (norm [delta_only [`%get_Type;`%Mkdtuple2?._1; `%return_either]; iota];
      // trefl (); -- TODO: this fails even if it is an equality.
      tadmit ())
   = QLambda (QIf QVar0 (QInl Qtt) (QInr Qtt))
 
 let test_match_either ()
-  : closed_exp_quotation ((qBool ^+ qBool) ^-> qBool) match_either
+  : ((qBool ^+ qBool) ^-> qBool) ⊩ match_either
   = QLambda (QCase QVar0 (QLambda #_ #_ #_ #(fun _ x -> x) QVar0) (QLambda #_ #_ #_ #(fun _ x -> x) QVar0))
 
 [@@ (preprocess_with simplify_qType)]
 let test_match_either' ()
-  : closed_exp_quotation ((qBool ^+ qBool) ^-> qBool) match_either'
+  : ((qBool ^+ qBool) ^-> qBool) ⊩ match_either'
   by (norm [delta_only [`%get_Type;`%Mkdtuple2?._1; `%match_either']; iota];
      dump "H";
      tadmit ()) // TODO: expected failure. any way to sort the cases?
   = QLambda (QCase QVar0 (QLambda #_ #_ #_ #(fun _ x -> x) QVar0) (QLambda #_ #_ #_ #(fun _ x -> x) QVar0))
 
 let test_match_either_arg ()
-  : closed_exp_quotation ((qBool ^+ qBool) ^-> qBool ^-> qBool) match_either_arg
+  : (((qBool ^+ qBool) ^-> qBool ^-> qBool) ⊩ match_either_arg)
   = QLambda (QLambda (
        QCase
          qVar1
